\documentclass{article}
\usepackage{color}
\usepackage{amsxtra}
\usepackage{amsthm}
\usepackage{amssymb}
\usepackage{amsfonts}

\begin{document}

\begin{equation}
	R_g^2 = \left< \frac{1}{N} \sum^{N}_{i=1} (\mathbf{r}_{i} - \mathbf{r}_{CM})^2 \right>
\end{equation}
\begin{equation}
	Q_{xy} = \frac{1}{N} \sum^{N}_{i=1} \mathbf{r}_x^i \mathbf{r}_y^i
\end{equation}
\begin{equation}
	Q = \left[  
		\begin{array}{ccc}
			Q_{xx} & Q_{xy} & Q_{xz} \\
			Q_{yx} & Q_{yy} & Q_{yz} \\
			Q_{zx} & Q_{zy} & Q_{zz}
		\end{array} 
	\right] 
	= \left[  
		\begin{array}{ccc}
			\lambda_{x}^2 & 0 & 0 \\
			0 & \lambda_{y}^2 & 0 \\
			0 & 0 & \lambda_{z}^2
		\end{array} 
	\right]
\end{equation}

\begin{equation}
	\lambda_{x}^2 \leq \lambda_{y}^2 \leq \lambda_{z}^2
\end{equation}
\begin{equation}
	b = \lambda_{z}^2 - \frac{1}{2}(\lambda_{x}^2 + \lambda_{y}^2)
\end{equation}
\begin{equation}
	c = \lambda_{y}^2 - \lambda_{x}^2
\end{equation}


\begin{equation}
	\kappa = \frac{3}{2}\frac{Tr\hat{Q}^2}{(TrQ)^2}
\end{equation}
\begin{equation}
	\hat{Q}_{ij} = Q_{ij} - \delta_{ij} TrQ/3
\end{equation}

\begin{equation}
	\kappa^2 = \frac{3}{2} \frac{\lambda_x^4 + \lambda_y^4 + \lambda_z^4}{(\lambda_x^2 + \lambda_y^2 + \lambda_z^2)^2} - \frac{1}{2}
\end{equation}
\begin{equation}
	0 \leq \kappa \leq 1
\end{equation}
\end{document}

